scripts/verify_cesk_gc_formal.sh
@@ -386,6 +386,8 @@ run_tlc "threading_end_to_end_safe" "ThreadingEndToEndInterleaving.tla" "MC_Thre
   pass ""
 run_tlc "threading_end_to_end_independent" "ThreadingEndToEndInterleaving.tla" "MC_ThreadingEndToEndInterleaving_independent.cfg" \
   pass ""
+run_tlc "threading_end_to_end_classification_no_shift" "ThreadingEndToEndInterleaving.tla" "MC_ThreadingEndToEndInterleaving_classification_no_shift.cfg" \
+  fail "The invariant of SchedulerClassificationRangesDisjoint is equal to FALSE"
 run_tlc "threading_end_to_end_active_fanout_missing_purity" "ThreadingEndToEndInterleaving.tla" "MC_ThreadingEndToEndInterleaving_active_fanout_missing_purity.cfg" \
   fail "The invariant of ActiveFanoutGateComplete is equal to FALSE"
 run_tlc "threading_end_to_end_active_fanout_missing_budget" "ThreadingEndToEndInterleaving.tla" "MC_ThreadingEndToEndInterleaving_active_fanout_missing_budget.cfg" \
